src/Lean/Meta/Tactic/Grind/Arith/IsRelevant.lean
@@ -6,15 +6,14 @@ Authors: Leonardo de Moura
 module
 prelude
 public import Lean.Meta.Tactic.Grind.Types
-import Lean.Meta.Tactic.Grind.Arith.Cutsat.ToInt
+import Lean.Meta.Tactic.Grind.Arith.Util
 import Lean.Meta.Tactic.Grind.Arith.Linear.StructId
 public section
 namespace Lean.Meta.Grind.Arith
 
 def isSupportedType (α  : Expr) : GoalM Bool := do
+  -- TODO: add support for new `toInt` and `toNat`.
   if isNatType α || isIntType α then
-    return true
-  else if (← Cutsat.getToIntId? α).isSome then
     return true
   else if (← Linear.getStructId? α).isSome then
     return true
